Remove l and v from AsMapsTo

src/goose_lang/lib/persistent_readonly.v
@@ -9,48 +9,47 @@ From Perennial.goose_lang Require Import proofmode.
 
 Section goose_lang.
   Context `{!invG Σ}.
-  Context {L V: Type}.
 
   Class AsMapsTo (P: iProp Σ)
-        (Φ : L -> Qp -> V -> iProp Σ) (l: L) (v: V) :=
-    { as_mapsto : P ≡ Φ l 1%Qp v;
-      as_mapsto_fractional :> forall l v, Fractional (λ q, Φ l q v);
-      as_mapsto_timeless :> forall l q v, Timeless (Φ l q v);
+        (Φ : Qp -> iProp Σ) :=
+    { as_mapsto : P ≡ Φ 1%Qp;
+      as_mapsto_fractional :> Fractional (λ q, Φ q);
+      as_mapsto_timeless :> ∀ q, Timeless (Φ q);
     }.
 
-  Arguments as_mapsto {P Φ l v} AsMapsTo.
+  Arguments as_mapsto {P Φ} AsMapsTo.
 
   Let N := nroot .@ "readonly".
 
-  Definition readonly_def P `{H: AsMapsTo P Φ l v}: iProp Σ :=
-    inv N (∃ (q: Qp), ⌜(Qcanon.Qclt q 1)%Qp⌝ ∗ Φ l q v).
+  Definition readonly_def P `{H: AsMapsTo P Φ}: iProp Σ :=
+    inv N (∃ (q: Qp), ⌜(Qcanon.Qclt q 1)%Qp⌝ ∗ Φ q).
   Definition readonly_aux : seal (@readonly_def). Proof. by eexists. Qed.
   Definition readonly := readonly_aux.(unseal).
   Definition readonly_eq : @readonly = @readonly_def := readonly_aux.(seal_eq).
-  Arguments readonly P {Φ}%function_scope {l v H}.
+  Arguments readonly P {Φ}%function_scope {H}.
 
   Ltac unseal := rewrite readonly_eq /readonly_def.
 
-  Theorem readonly_alloc P `{H: AsMapsTo P Φ l v} (q:Qp) E :
+  Theorem readonly_alloc P `{H: AsMapsTo P Φ} (q:Qp) E :
     Qcanon.Qclt q 1 ->
-    Φ l q v ={E}=∗ readonly P.
+    Φ q ={E}=∗ readonly P.
   Proof.
     unseal.
     iIntros (Hbound) "HP".
     iMod (inv_alloc with "[HP]") as "$"; auto.
   Qed.
 
-  Global Instance readonly_persistent P `{H: AsMapsTo P Φ l v} : Persistent (readonly P).
+  Global Instance readonly_persistent P `{H: AsMapsTo P Φ} : Persistent (readonly P).
   Proof. unseal; apply _. Qed.
 
-  Instance as_mapsto_AsFractional P `{H: AsMapsTo P Φ l v} :
-    AsFractional (Φ l q v) (λ q, Φ l q v) q.
+  Instance as_mapsto_AsFractional P `{H: AsMapsTo P Φ} :
+    AsFractional (Φ q) (λ q, Φ q) q.
   Proof.
     split; auto.
     apply _.
   Qed.
 
-  Theorem readonly_alloc_1 P `{H: AsMapsTo P Φ l v} E :
+  Theorem readonly_alloc_1 P `{H: AsMapsTo P Φ} E :
     P ={E}=∗ readonly P.
   Proof.
     iIntros "HP".
@@ -60,15 +59,15 @@ Section goose_lang.
     reflexivity.
   Qed.
 
-  Theorem readonly_load_lt P `{H: AsMapsTo P Φ l v} E :
+  Theorem readonly_load_lt P `{H: AsMapsTo P Φ} E :
     ↑N ⊆ E ->
-    readonly P ={E}=∗ ∃ (q: Qp), ⌜(Qcanon.Qclt q 1)%Qc⌝ ∗ Φ l q v.
+    readonly P ={E}=∗ ∃ (q: Qp), ⌜(Qcanon.Qclt q 1)%Qc⌝ ∗ Φ q.
   Proof.
     iIntros (Hsub) "Hro".
     unseal.
-    assert (Timeless (∃ q, Φ l q v)).
+    assert (Timeless (∃ q, Φ q)).
     { apply _. }
-    iMod (inv_dup_acc (∃ (q: Qp), ⌜(Qcanon.Qclt q 1)%Qc⌝ ∗ Φ l q v) with "Hro []") as ">H"; first by auto.
+    iMod (inv_dup_acc (∃ (q: Qp), ⌜(Qcanon.Qclt q 1)%Qc⌝ ∗ Φ q) with "Hro []") as ">H"; first by auto.
     { iIntros "HΦ".
       iDestruct "HΦ" as (q) "[% HΦ]".
       iDestruct (fractional_half with "HΦ") as "[HΦ1 HΦ2]".
@@ -81,9 +80,9 @@ Section goose_lang.
     auto.
   Qed.
 
-  Theorem readonly_load P `{H: AsMapsTo P Φ l v} E :
+  Theorem readonly_load P `{H: AsMapsTo P Φ} E :
     ↑N ⊆ E ->
-    readonly P ={E}=∗ ∃ q, Φ l q v.
+    readonly P ={E}=∗ ∃ q, Φ q.
   Proof.
     iIntros (Hsub) "Hro".
     iMod (readonly_load_lt with "Hro") as (q) "[% HΦ]"; auto.
@@ -93,16 +92,16 @@ End goose_lang.
 
 Instance heap_mapsto_AsMapsTo `{ext: !ext_op} `{!na_heapG loc val Σ}
          (l: loc) (v: val) :
-  AsMapsTo (l ↦ v) (λ l q v, l ↦{q} v)%I l v.
+  AsMapsTo (l ↦ v) (λ q, l ↦{q} v)%I.
 Proof.
   split; [done|apply _|apply _].
 Qed.
 
-Instance mapsto_AsMapsTo `{ffi_sem: ext_semantics} `(hG: gen_heapG L V Σ) l v :
-  AsMapsTo (mapsto (hG:=hG) l 1 v) (λ l q v, mapsto (hG:=hG) l q v) l v.
+Instance mapsto_AsMapsTo `{ffi_sem: ext_semantics} `(hG: gen_heapG Σ) :
+  AsMapsTo (mapsto (hG:=hG) l 1 v) (λ q, mapsto (hG:=hG) l q v).
 Proof.
   split; [done|apply _|apply _].
 Qed.
 
-Hint Mode AsMapsTo - - - + - - - : typeclass_instances.
-Arguments readonly {Σ invG0} {L V}%type_scope _%bi_scope {Φ}%function_scope {l v H}.
+Hint Mode AsMapsTo - + - : typeclass_instances.
+Arguments readonly {Σ invG0} _%bi_scope {Φ}%function_scope {H}.
